WIP

Clap/eDSLState/Circuit.lean
@@ -1,18 +1,18 @@
 import Mathlib.Control.Monad.Writer
 
-import Clap.eDSLState.Exp
+import Clap.eDSLState.HashCons.CacheExpr
+import Clap.eDSLState.HashCons.Eval
 import Clap.eDSLState.Varstore
 
 namespace Clap
 
 @[grind cases]
 inductive CircuitusPlanus (p : ℕ) where
-  | eq0 (e : FixedExp p)
+  | eq0 (e : HashConsM p ExprRef)
   | lam
-  | share (e : FixedExp p)
-  | isZero (e : FixedExp p)
-  | num2bits (w : ℕ) (e : FixedExp p)
-  deriving Repr
+  | share (e : HashConsM p ExprRef)
+  | isZero (e : HashConsM p ExprRef)
+  | num2bits (w : ℕ) (e : HashConsM p ExprRef)
 
 abbrev CircuitState (p : ℕ) := Array (CircuitusPlanus p)
 
@@ -40,7 +40,7 @@ section
 
 -- TODO do we need all of these?
 variable {p k numAlloc : ℕ} {result result' : CircuitResult p}
-         {constraint : Prop} {vars : Vector (ZMod p) k} {e : FixedExp p}
+         {constraint : Prop} {vars : Vector (ZMod p) k} {e : HashConsM p ExprRef}
          {varStore : VarStore p}
 
 def init (p : ℕ) : CircuitResult p := ⟨0, ∅, True⟩
@@ -89,46 +89,47 @@ lemma varStore_addConstraint : (result.addConstraint constraint).varStore = resu
 lemma constraints_addConstraint : (result.addConstraint constraint).constraints =
                                   (result.constraints ∧ constraint) := rfl
 
-def allocAnonymous (result : CircuitResult p) : CircuitResult p :=
-  {result with numAlloc := result.numAlloc + 1}
+def allocAnonymous (result : CircuitResult p) : HashConsM p (CircuitResult p) :=
+  return {result with numAlloc := result.numAlloc + 1}
 
-@[simp, grind =]
-lemma allocAnonymous_mk
-  (numAlloc : ℕ)
-  (varStore : VarStore p)
-  (constraints : Prop)
-:
-  (Edsl.CircuitResult.mk numAlloc varStore constraints).allocAnonymous =
-  Edsl.CircuitResult.mk (numAlloc + 1) varStore constraints
-:= rfl
+-- @[simp, grind =]
+-- lemma allocAnonymous_mk
+--   (numAlloc : ℕ)
+--   (varStore : VarStore p)
+--   (constraints : Prop)
+-- :
+--   (Edsl.CircuitResult.mk numAlloc varStore constraints).allocAnonymous =
+--   Edsl.CircuitResult.mk (numAlloc + 1) varStore constraints
+-- := rfl
 
-@[simp, grind =]
-lemma allocAnonymous_unconstrained :
-  unconstrained[numAlloc][varStore].allocAnonymous =
-  ⟨numAlloc + 1, varStore, True⟩ := by rfl
+-- @[simp, grind =]
+-- lemma allocAnonymous_unconstrained :
+--   unconstrained[numAlloc][varStore].allocAnonymous =
+--   ⟨numAlloc + 1, varStore, True⟩ := by rfl
 
-@[simp, grind =]
-lemma numAlloc_allocAnonymous : result.allocAnonymous.numAlloc = result.numAlloc + 1 := rfl
+-- @[simp, grind =]
+-- lemma numAlloc_allocAnonymous : result.allocAnonymous.numAlloc = result.numAlloc + 1 := rfl
 
-@[simp, grind =]
-lemma varStore_allocAnonymous : result.allocAnonymous.varStore = result.varStore := rfl
+-- @[simp, grind =]
+-- lemma varStore_allocAnonymous : result.allocAnonymous.varStore = result.varStore := rfl
 
-@[simp, grind =]
-lemma constraints_allocAnonymous : result.allocAnonymous.constraints = result.constraints := rfl
+-- @[simp, grind =]
+-- lemma constraints_allocAnonymous : result.allocAnonymous.constraints = result.constraints := rfl
 
 @[grind =]
-def get? (result : CircuitResult p) (e : FixedExp p) : Option (ZMod p) :=
-  e.eval result.varStore
+def get? (result : CircuitResult p) (e : HashConsM p ExprRef) : HashConsM p (Option (ZMod p)) :=
+  HashConsM.eval result.varStore e
 
-instance : Membership (FixedExp p) (CircuitResult p) := ⟨fun Γ x ↦ (get? Γ x).isSome⟩
+-- instance : Membership (HashConsM p ExprRef) (HashConsM p (CircuitResult p)) :=
+--   ⟨fun Γ x ↦ (get? Γ x).isSome⟩
 
-instance : GetElem (CircuitResult p) (FixedExp p) (ZMod p) (fun Γ x ↦ x ∈ Γ) :=
-  ⟨fun Γ x h ↦ Γ.get? x |>.get h⟩
+-- instance : GetElem (CircuitResult p) (CacheExpr p) (ZMod p) (fun Γ x ↦ x ∈ Γ) :=
+--   ⟨fun Γ x h ↦ Γ.get? x |>.get h⟩
 
 
 @[simp, grind =]
 lemma get?_mk
-  (e : FixedExp p)
+  (e : HashConsM p ExprRef)
   (numAlloc : ℕ)
   (varStore : VarStore p)
   (constraints : Prop)
@@ -141,51 +142,55 @@ lemma get?_mk
 lemma get?_of_varStore_eq_varStore (h : result.varStore = result'.varStore) : result.get? e = result'.get? e := by
   simp_all [CircuitResult.get?]
 
-def getD (result : CircuitResult p) (e : FixedExp p) :=
-  result.get? e |>.getD 0
+def getD (result : CircuitResult p) (e : HashConsM p ExprRef) : HashConsM p (ZMod p) := do
+  result.get? e <&> Option.getD (dflt := 0)
 
-instance {p} : GetElem? (CircuitResult p) (FixedExp p) (ZMod p) (fun Γ x ↦ x ∈ Γ) :=
-  ⟨get?, getD⟩
+-- instance {p} : GetElem? (CircuitResult p) (HashConsM p ExprRef) (ZMod p) (fun Γ x ↦ x ∈ Γ) :=
+--   ⟨get?, getD⟩
 
 @[simp, grind =]
-lemma getD_eq_get?_getD : result.getD e = (result.get? e |>.getD 0) := rfl
+lemma getD_eq_get?_getD : result.getD e = result.get? e <&> Option.getD (dflt := 0) := rfl
 
 @[simp, grind =]
 lemma get?_unconstrained :
   unconstrained[numAlloc][varStore].get? e =
   [varStore|e] := by simp [unconstrained]
 
-def assertAllocated (result : CircuitResult p) (e : FixedExp p) : CircuitResult p :=
-  result.addConstraint (result.get? e).isSome
+def assertAllocated (result : CircuitResult p) (e : HashConsM p ExprRef) : HashConsM p (CircuitResult p) := do
+  let val ← result.get? e
+  return result.addConstraint val.isSome
 
 @[simp, grind =]
 lemma assertAllocated_mk
-  (e : FixedExp p)
+  (e : HashConsM p ExprRef)
   (numAlloc : ℕ)
   (varStore : VarStore p)
   (constraints : Prop)
 :
-  (Edsl.CircuitResult.mk numAlloc varStore constraints).assertAllocated e =
-  Edsl.CircuitResult.mk numAlloc varStore (constraints ∧ e ∈ varStore)
-:= rfl
+  (Edsl.CircuitResult.mk numAlloc varStore constraints).assertAllocated e = sorry
+  -- Edsl.CircuitResult.mk numAlloc varStore (constraints ∧ _)
+:= by
+  unfold assertAllocated
+  simp
+  sorry
 
-@[simp, grind =]
-lemma numAlloc_assertAllocated :
-  (result.assertAllocated e).numAlloc = result.numAlloc := rfl
+-- @[simp, grind =]
+-- lemma numAlloc_assertAllocated :
+--   (result.assertAllocated e).numAlloc = result.numAlloc := rfl
 
-@[simp, grind =]
-lemma varStore_assertAllocated :
-  (result.assertAllocated e).varStore = result.varStore := rfl
+-- @[simp, grind =]
+-- lemma varStore_assertAllocated :
+--   (result.assertAllocated e).varStore = result.varStore := rfl
 
-@[simp, grind =]
-lemma constraints_assertAllocated :
-  (result.assertAllocated e).constraints = (result.constraints ∧ (result.get? e).isSome = true) := rfl
+-- @[simp, grind =]
+-- lemma constraints_assertAllocated :
+--   (result.assertAllocated e).constraints = (result.constraints ∧ (result.get? e).isSome = true) := rfl
 
-@[simp, grind =]
-lemma assertAllocated_unconstrained :
-  unconstrained[numAlloc][varStore].assertAllocated e =
-  letI α := unconstrained[numAlloc][varStore]
-  α.addConstraint (e ∈ α) := rfl
+-- @[simp, grind =]
+-- lemma assertAllocated_unconstrained :
+--   unconstrained[numAlloc][varStore].assertAllocated e =
+--   letI α := unconstrained[numAlloc][varStore]
+--   α.addConstraint (e ∈ α) := rfl
 
 def alloc {k p : ℕ} (result : CircuitResult p) (vals : Vector (ZMod p) k) : CircuitResult p :=
   let indexed := (Vector.range k).map (·+result.numAlloc) |>.zip vals
@@ -219,417 +224,423 @@ lemma varStore_alloc {vars : Vector (ZMod p) k} :
 lemma constraints_alloc {vars : Vector (ZMod p) k} :
   (result.alloc vars).constraints = result.constraints := rfl
 
-def step (result : CircuitResult p) (next : CircuitusPlanus p) : CircuitResult p :=
+def step (result : CircuitResult p) (next : CircuitusPlanus p) : HashConsM p (CircuitResult p) :=
   -- dbg_trace s!"running: {repr next}"
   match next with
-  | .eq0 e => result.addConstraint (result.get? e = .some 0)
+  | .eq0 e => do
+    let x ← result.get? e
+    return result.addConstraint (x = .some 0)
   | .lam => result.allocAnonymous
-  | .share e =>
-    dbg_trace s!"sharing an expression of size: {e.size}"
-    result.assertAllocated e |>.alloc #v[result.getD e]
-  | .isZero e => result.assertAllocated e |>.alloc #v[if result.get? e = .some 0 then 1 else 0]
-  | .num2bits width e => result.assertAllocated e |>.alloc (num2bitsLsbPureV width (result.getD e))
+  | .share e => do
+    let result' ← Clap.Edsl.CircuitResult.assertAllocated result e
+    return alloc result' #v[←result.getD e]
+  | .isZero e => do
+    let result' ← Clap.Edsl.CircuitResult.assertAllocated result e
+    return alloc result' #v[if (←result.get? e) = .some 0 then 1 else 0]
+  | .num2bits width e => do
+    let result' ← Clap.Edsl.CircuitResult.assertAllocated result e
+    return alloc result' (num2bitsLsbPureV width (←result.getD e))
 
-notation "[" σ "|" cmd "]ₛ" => step σ cmd
+-- notation "[" σ "|" cmd "]ₛ" => step σ cmd
 
--- TODO do we want to make individual functions for these parts and prove properties about them
-@[simp, grind =]
-lemma step_mk
-  (numAlloc : ℕ)
-  (varStore : VarStore p)
-  (constraints : Prop)
-  (next : CircuitusPlanus p)
-: (Edsl.CircuitResult.mk numAlloc varStore constraints).step next =
-  Edsl.CircuitResult.mk
-    (match next with
-      | .eq0 _ => numAlloc
-      | .lam => numAlloc + 1
-      | .share e => numAlloc + 1
-      | .isZero e => numAlloc + 1
-      | .num2bits width _ => numAlloc + width
-    )
-    (match next with
-      | .eq0 _ => varStore
-      | .lam => varStore
-      | .share e => varStore.insert numAlloc ((e.eval varStore).getD 0)
-      | .isZero e => varStore.insert numAlloc (if (e.eval varStore) = .some 0 then 1 else 0)
-      | .num2bits width e => varStore.insertMany
-        ((Vector.map (fun x => x + numAlloc) (Vector.range width)).zip
-          (num2bitsLsbPureV width ((FixedExp.eval varStore e).getD 0)))
-    )
-    (match next with
-      | .eq0 e => constraints ∧ (e.eval varStore) = .some 0
-      | .lam => constraints
-      | .share e => constraints ∧ (e.eval varStore).isSome
-      | .isZero e => constraints ∧ (e.eval varStore).isSome
-      | .num2bits width e => constraints ∧ (e.eval varStore).isSome
-    )
-:= by
-  sorry
-  -- cases next <;> simp [CircuitResult.step, Membership.mem]
-  -- rfl
+-- -- TODO do we want to make individual functions for these parts and prove properties about them
+-- @[simp, grind =]
+-- lemma step_mk
+--   (numAlloc : ℕ)
+--   (varStore : VarStore p)
+--   (constraints : Prop)
+--   (next : CircuitusPlanus p)
+-- : (Edsl.CircuitResult.mk numAlloc varStore constraints).step next =
+--   Edsl.CircuitResult.mk
+--     (match next with
+--       | .eq0 _ => numAlloc
+--       | .lam => numAlloc + 1
+--       | .share e => numAlloc + 1
+--       | .isZero e => numAlloc + 1
+--       | .num2bits width _ => numAlloc + width
+--     )
+--     (match next with
+--       | .eq0 _ => varStore
+--       | .lam => varStore
+--       | .share e => varStore.insert numAlloc ((e.eval varStore).getD 0)
+--       | .isZero e => varStore.insert numAlloc (if (e.eval varStore) = .some 0 then 1 else 0)
+--       | .num2bits width e => varStore.insertMany
+--         ((Vector.map (fun x => x + numAlloc) (Vector.range width)).zip
+--           (num2bitsLsbPureV width ((FixedExp.eval varStore e).getD 0)))
+--     )
+--     (match next with
+--       | .eq0 e => constraints ∧ (e.eval varStore) = .some 0
+--       | .lam => constraints
+--       | .share e => constraints ∧ (e.eval varStore).isSome
+--       | .isZero e => constraints ∧ (e.eval varStore).isSome
+--       | .num2bits width e => constraints ∧ (e.eval varStore).isSome
+--     )
+-- := by
+--   sorry
+--   -- cases next <;> simp [CircuitResult.step, Membership.mem]
+--   -- rfl
+
+-- -- @[simp, grind =]
+-- lemma step_unconstrained {command : CircuitusPlanus p} :
+--   [unconstrained[numAlloc][varStore]|command]ₛ =
+--   [⟨numAlloc, varStore, True⟩|command]ₛ := rfl
+
+-- def split (result : CircuitResult p) : CircuitResult p :=
+--   {result with constraints := True}
 
 -- @[simp, grind =]
-lemma step_unconstrained {command : CircuitusPlanus p} :
-  [unconstrained[numAlloc][varStore]|command]ₛ =
-  [⟨numAlloc, varStore, True⟩|command]ₛ := rfl
+-- lemma numAlloc_split : result.split.numAlloc = result.numAlloc := rfl
 
-def split (result : CircuitResult p) : CircuitResult p :=
-  {result with constraints := True}
+-- @[simp, grind =]
+-- lemma varStore_split : result.split.varStore = result.varStore := rfl
 
-@[simp, grind =]
-lemma numAlloc_split : result.split.numAlloc = result.numAlloc := rfl
+-- @[simp, grind =]
+-- lemma constraints_split : result.split.constraints = True := rfl
 
-@[simp, grind =]
-lemma varStore_split : result.split.varStore = result.varStore := rfl
+-- section
 
-@[simp, grind =]
-lemma constraints_split : result.split.constraints = True := rfl
+-- variable {p width : ℕ} {result : CircuitResult p} {e : FixedExp p}
 
-section
+-- @[simp, grind =]
+-- lemma step_eq0 :
+--   [result|.eq0 e]ₛ = result.addConstraint (result[e]? = .some 0) := rfl
 
-variable {p width : ℕ} {result : CircuitResult p} {e : FixedExp p}
+-- @[simp, grind =]
+-- lemma step_lam :
+--   [result|.lam]ₛ = result.allocAnonymous := rfl
 
-@[simp, grind =]
-lemma step_eq0 :
-  [result|.eq0 e]ₛ = result.addConstraint (result[e]? = .some 0) := rfl
+-- @[simp, grind =]
+-- lemma step_share :
+--   [result|.share e]ₛ = (result.assertAllocated e |>.alloc #v[result.getD e]) := rfl
 
-@[simp, grind =]
-lemma step_lam :
-  [result|.lam]ₛ = result.allocAnonymous := rfl
+-- @[simp, grind =]
+-- lemma step_isZero :
+--   [result|.isZero e]ₛ = (result.assertAllocated e |>.alloc #v[if result[e]? = .some 0 then 1 else 0]) := rfl
 
-@[simp, grind =]
-lemma step_share :
-  [result|.share e]ₛ = (result.assertAllocated e |>.alloc #v[result.getD e]) := rfl
+-- @[simp, grind =]
+-- lemma step_num2bits :
+--   [result|.num2bits width e]ₛ = (result.assertAllocated e |>.alloc (num2bitsLsbPureV width result[e]!)) := rfl
 
-@[simp, grind =]
-lemma step_isZero :
-  [result|.isZero e]ₛ = (result.assertAllocated e |>.alloc #v[if result[e]? = .some 0 then 1 else 0]) := rfl
+-- lemma addConstraint_eq_mk :
+--   result.addConstraint constraint =
+--   ⟨result.numAlloc, result.varStore, result.constraints ∧ constraint⟩ := rfl
 
-@[simp, grind =]
-lemma step_num2bits :
-  [result|.num2bits width e]ₛ = (result.assertAllocated e |>.alloc (num2bitsLsbPureV width result[e]!)) := rfl
+-- lemma allocAnonymous_eq_mk :
+--   result.allocAnonymous =
+--   ⟨result.numAlloc + 1, result.varStore, result.constraints⟩ := rfl
 
-lemma addConstraint_eq_mk :
-  result.addConstraint constraint =
-  ⟨result.numAlloc, result.varStore, result.constraints ∧ constraint⟩ := rfl
+-- lemma alloc_eq_mk {k} {vals : Vector _ k} :
+--   result.alloc vals =
+--   ⟨result.numAlloc + k,
+--    result.varStore.insertMany (((Vector.range k).map (· + result.numAlloc)).zip vals),
+--    result.constraints⟩ := by rfl
 
-lemma allocAnonymous_eq_mk :
-  result.allocAnonymous =
-  ⟨result.numAlloc + 1, result.varStore, result.constraints⟩ := rfl
+-- lemma assertAllocated_eq_addConstraint :
+--   result.assertAllocated e = result.addConstraint (e ∈ result) := rfl
 
-lemma alloc_eq_mk {k} {vals : Vector _ k} :
-  result.alloc vals =
-  ⟨result.numAlloc + k,
-   result.varStore.insertMany (((Vector.range k).map (· + result.numAlloc)).zip vals),
-   result.constraints⟩ := by rfl
+-- end
 
-lemma assertAllocated_eq_addConstraint :
-  result.assertAllocated e = result.addConstraint (e ∈ result) := rfl
+-- end
 
-end
+-- end CircuitResult
 
-end
+abbrev CircuitState.evalInOrder {p : ℕ} (circuit : CircuitState p) := circuit.foldlM CircuitResult.step
 
-end CircuitResult
+-- def CircuitState.eval {p : ℕ} (circuit : CircuitState p) (varStore : VarStore p) (numAlloc : ℕ) : CircuitResult p :=
+--   CircuitState.evalInOrder circuit ⟨numAlloc, varStore, True⟩
 
-abbrev CircuitState.evalInOrder {p : ℕ} (circuit : CircuitState p) := circuit.foldl CircuitResult.step
+-- notation "[" varStore ", " numAlloc "|" circuit "]ₑ" => CircuitState.eval circuit varStore numAlloc
 
-def CircuitState.eval {p : ℕ} (circuit : CircuitState p) (varStore : VarStore p) (numAlloc : ℕ) : CircuitResult p :=
-  CircuitState.evalInOrder circuit ⟨numAlloc, varStore, True⟩
+-- namespace CircuitResult
 
-notation "[" varStore ", " numAlloc "|" circuit "]ₑ" => CircuitState.eval circuit varStore numAlloc
+-- variable {p : ℕ}
 
-namespace CircuitResult
+-- @[ext, grind ext]
+-- lemma ext {p : ℕ} {r1 r2 : CircuitResult p}
+--   (h_numAlloc : r1.numAlloc = r2.numAlloc)
+--   (h_varStore : r1.varStore = r2.varStore)
+--   (h_constraints : r1.constraints = r2.constraints)
+-- :
+--   r1 = r2
+-- := by
+--   obtain ⟨a1, b1, c1⟩ := r1
+--   obtain ⟨a2, b2, c2⟩ := r2
+--   simp_all
 
-variable {p : ℕ}
+-- lemma foldl_step_numAlloc_independent_of_constraints
+--   {numAlloc : ℕ}
+--   {varStore : VarStore p}
+--   {constraints1 constraints2 : Prop}
+--   {circuit : CircuitState p}
+-- :
+--   (CircuitState.evalInOrder circuit ⟨numAlloc, varStore, constraints1⟩).numAlloc =
+--   (CircuitState.evalInOrder circuit ⟨numAlloc, varStore, constraints2⟩).numAlloc
+-- := by
+--   rcases circuit with ⟨circuit⟩
+--   simp only [List.size_toArray, List.foldl_toArray']
+--   rewrite [←List.reverse_reverse circuit]
+--   induction circuit.reverse <;> grind
 
-@[ext, grind ext]
-lemma ext {p : ℕ} {r1 r2 : CircuitResult p}
-  (h_numAlloc : r1.numAlloc = r2.numAlloc)
-  (h_varStore : r1.varStore = r2.varStore)
-  (h_constraints : r1.constraints = r2.constraints)
-:
-  r1 = r2
-:= by
-  obtain ⟨a1, b1, c1⟩ := r1
-  obtain ⟨a2, b2, c2⟩ := r2
-  simp_all
+-- @[grind =>]
+-- lemma foldr_step_numAlloc_independent_of_constraints
+--   {numAlloc : ℕ}
+--   {varStore : VarStore p}
+--   {constraints1 constraints2 : Prop}
+--   {circuit : CircuitState p}
+-- :
+--   (Array.foldr (λ x y => step y x) ⟨numAlloc, varStore, constraints1⟩ circuit).numAlloc =
+--   (Array.foldr (λ x y => step y x) ⟨numAlloc, varStore, constraints2⟩ circuit).numAlloc
+-- := by
+--   rcases circuit with ⟨circuit⟩
+--   rewrite [←List.reverse_reverse circuit]
+--   rw [show Array.mk circuit.reverse.reverse = Array.reverse ⟨circuit.reverse⟩ by simp]
+--   simp only [Array.foldr_reverse]
+--   exact foldl_step_numAlloc_independent_of_constraints
 
-lemma foldl_step_numAlloc_independent_of_constraints
-  {numAlloc : ℕ}
-  {varStore : VarStore p}
-  {constraints1 constraints2 : Prop}
-  {circuit : CircuitState p}
-:
-  (CircuitState.evalInOrder circuit ⟨numAlloc, varStore, constraints1⟩).numAlloc =
-  (CircuitState.evalInOrder circuit ⟨numAlloc, varStore, constraints2⟩).numAlloc
-:= by
-  rcases circuit with ⟨circuit⟩
-  simp only [List.size_toArray, List.foldl_toArray']
-  rewrite [←List.reverse_reverse circuit]
-  induction circuit.reverse <;> grind
+-- lemma foldl_step_varStore_independent_of_constraints
+--   {numAlloc : ℕ}
+--   {varStore : VarStore p}
+--   {constraints1 constraints2 : Prop}
+--   {circuit : CircuitState p}
+-- :
+--   (circuit.foldl step ⟨numAlloc, varStore, constraints1⟩).varStore =
+--   (circuit.foldl step ⟨numAlloc, varStore, constraints2⟩).varStore
+-- := by
+--   rcases circuit with ⟨circuit⟩
+--   rewrite [←List.reverse_reverse circuit]
+--   induction circuit.reverse
+--   -- TODO This used to be just `induction <;> grind`, now we need lemmas in terms of `GetElem?`
+--   -- to push through
+--   grind [=GetElem?.getElem?]
+--   simp
+--   next hd tl ih =>
+--     simp at *
+--     rcases hd with _ | _ | _ | _ | _
+--     · grind
+--     · grind
+--     · rw [Array.foldr_toList, Array.foldr_toList]
+--       grind
+--     · rw [Array.foldr_toList, Array.foldr_toList]
+--       simp only [step_isZero]
+--       unfold GetElem?.getElem?
+--       unfold instGetElem?FixedExpZModMem
+--       grind [GetElem?.getElem?, instGetElem?FixedExpZModMem]
+--     · 
+--       simp
+--       unfold GetElem?.getElem!
+--       unfold instGetElem?FixedExpZModMem
+--       simp
+--       rw [Array.foldr_toList, Array.foldr_toList]
+--       grind
 
-@[grind =>]
-lemma foldr_step_numAlloc_independent_of_constraints
-  {numAlloc : ℕ}
-  {varStore : VarStore p}
-  {constraints1 constraints2 : Prop}
-  {circuit : CircuitState p}
-:
-  (Array.foldr (λ x y => step y x) ⟨numAlloc, varStore, constraints1⟩ circuit).numAlloc =
-  (Array.foldr (λ x y => step y x) ⟨numAlloc, varStore, constraints2⟩ circuit).numAlloc
-:= by
-  rcases circuit with ⟨circuit⟩
-  rewrite [←List.reverse_reverse circuit]
-  rw [show Array.mk circuit.reverse.reverse = Array.reverse ⟨circuit.reverse⟩ by simp]
-  simp only [Array.foldr_reverse]
-  exact foldl_step_numAlloc_independent_of_constraints
+-- @[grind .]
+-- lemma foldr_step_varStore_independent_of_constraints
+--   {numAlloc : ℕ}
+--   {varStore : VarStore p}
+--   {constraints1 constraints2 : Prop}
+--   {circuit : CircuitState p}
+-- :
+--   (Array.foldr (λ x y => step y x) ⟨numAlloc, varStore, constraints1⟩ circuit).varStore =
+--   (Array.foldr (λ x y => step y x) ⟨numAlloc, varStore, constraints2⟩ circuit).varStore
+-- := by
+--   rcases circuit with ⟨circuit⟩
+--   rewrite [←List.reverse_reverse circuit]
+--   rw [show Array.mk circuit.reverse.reverse = Array.reverse ⟨circuit.reverse⟩ by simp]
+--   simp only [Array.foldr_reverse]
+--   exact foldl_step_varStore_independent_of_constraints
 
-lemma foldl_step_varStore_independent_of_constraints
-  {numAlloc : ℕ}
-  {varStore : VarStore p}
-  {constraints1 constraints2 : Prop}
-  {circuit : CircuitState p}
-:
-  (circuit.foldl step ⟨numAlloc, varStore, constraints1⟩).varStore =
-  (circuit.foldl step ⟨numAlloc, varStore, constraints2⟩).varStore
-:= by
-  rcases circuit with ⟨circuit⟩
-  rewrite [←List.reverse_reverse circuit]
-  induction circuit.reverse
-  -- TODO This used to be just `induction <;> grind`, now we need lemmas in terms of `GetElem?`
-  -- to push through
-  grind [=GetElem?.getElem?]
-  simp
-  next hd tl ih =>
-    simp at *
-    rcases hd with _ | _ | _ | _ | _
-    · grind
-    · grind
-    · rw [Array.foldr_toList, Array.foldr_toList]
-      grind
-    · rw [Array.foldr_toList, Array.foldr_toList]
-      simp only [step_isZero]
-      unfold GetElem?.getElem?
-      unfold instGetElem?FixedExpZModMem
-      grind [GetElem?.getElem?, instGetElem?FixedExpZModMem]
-    · 
-      simp
-      unfold GetElem?.getElem!
-      unfold instGetElem?FixedExpZModMem
-      simp
-      rw [Array.foldr_toList, Array.foldr_toList]
-      grind
+-- /--
+-- This exists to appease `grind`.
+-- -/
+-- @[grind! .]
+-- lemma foldr_step_varStore_independent_of_constraints'
+--   {circuit : CircuitState p}
+--   {σ₁ σ₂ : CircuitResult p}
+--   (h₁ : σ₁.numAlloc = σ₂.numAlloc)
+--   (h₂ : σ₁.varStore = σ₂.varStore)
+-- :
+--   (Array.foldr (λ x y => step y x) σ₁ circuit).varStore =
+--   (Array.foldr (λ x y => step y x) σ₂ circuit).varStore
+-- := by
+--   rewrite [←Array.reverse_reverse circuit]
+--   simp only [Array.foldr_reverse]
+--   grind [cases CircuitResult]
 
-@[grind .]
-lemma foldr_step_varStore_independent_of_constraints
-  {numAlloc : ℕ}
-  {varStore : VarStore p}
-  {constraints1 constraints2 : Prop}
-  {circuit : CircuitState p}
-:
-  (Array.foldr (λ x y => step y x) ⟨numAlloc, varStore, constraints1⟩ circuit).varStore =
-  (Array.foldr (λ x y => step y x) ⟨numAlloc, varStore, constraints2⟩ circuit).varStore
-:= by
-  rcases circuit with ⟨circuit⟩
-  rewrite [←List.reverse_reverse circuit]
-  rw [show Array.mk circuit.reverse.reverse = Array.reverse ⟨circuit.reverse⟩ by simp]
-  simp only [Array.foldr_reverse]
-  exact foldl_step_varStore_independent_of_constraints
+-- lemma foldl_step_constraints_and
+--   {result : CircuitResult p}
+--   {circuit : CircuitState p}
+-- :
+--   (CircuitState.evalInOrder circuit result).constraints = (
+--     result.constraints ∧
+--     (CircuitState.evalInOrder circuit result.split).constraints
+--   )
+-- := by
+--   rcases circuit with ⟨circuit⟩
+--   rewrite [←List.reverse_reverse circuit]
+--   induction circuit.reverse
+--   -- TODO This used to be just `induction <;> grind`, now we need lemmas in terms of `GetElem?`
+--   -- to push through
+--   grind
+--   simp
+--   next hd tl ih =>
+--     simp at *
+--     rcases hd with _ | _ | _ | _ | _
+--     · 
+--       simp
+--       unfold GetElem?.getElem?
+--       unfold instGetElem?FixedExpZModMem
+--       rw [Array.foldr_toList, Array.foldr_toList]
+--       grind [GetElem?.getElem?, instGetElem?FixedExpZModMem]
+--     · grind
+--     · rw [Array.foldr_toList, Array.foldr_toList]
+--       grind
+--     · simp only [step_isZero]
+--       unfold GetElem?.getElem?
+--       unfold instGetElem?FixedExpZModMem
+--       rw [Array.foldr_toList, Array.foldr_toList]
+--       grind [GetElem?.getElem?, instGetElem?FixedExpZModMem]
+--     · simp
+--       unfold get?
+--       rw [Array.foldr_toList, Array.foldr_toList]
+--       grind
 
-/--
-This exists to appease `grind`.
--/
-@[grind! .]
-lemma foldr_step_varStore_independent_of_constraints'
-  {circuit : CircuitState p}
-  {σ₁ σ₂ : CircuitResult p}
-  (h₁ : σ₁.numAlloc = σ₂.numAlloc)
-  (h₂ : σ₁.varStore = σ₂.varStore)
-:
-  (Array.foldr (λ x y => step y x) σ₁ circuit).varStore =
-  (Array.foldr (λ x y => step y x) σ₂ circuit).varStore
-:= by
-  rewrite [←Array.reverse_reverse circuit]
-  simp only [Array.foldr_reverse]
-  grind [cases CircuitResult]
-
-lemma foldl_step_constraints_and
-  {result : CircuitResult p}
-  {circuit : CircuitState p}
-:
-  (CircuitState.evalInOrder circuit result).constraints = (
-    result.constraints ∧
-    (CircuitState.evalInOrder circuit result.split).constraints
-  )
-:= by
-  rcases circuit with ⟨circuit⟩
-  rewrite [←List.reverse_reverse circuit]
-  induction circuit.reverse
-  -- TODO This used to be just `induction <;> grind`, now we need lemmas in terms of `GetElem?`
-  -- to push through
-  grind
-  simp
-  next hd tl ih =>
-    simp at *
-    rcases hd with _ | _ | _ | _ | _
-    · 
-      simp
-      unfold GetElem?.getElem?
-      unfold instGetElem?FixedExpZModMem
-      rw [Array.foldr_toList, Array.foldr_toList]
-      grind [GetElem?.getElem?, instGetElem?FixedExpZModMem]
-    · grind
-    · rw [Array.foldr_toList, Array.foldr_toList]
-      grind
-    · simp only [step_isZero]
-      unfold GetElem?.getElem?
-      unfold instGetElem?FixedExpZModMem
-      rw [Array.foldr_toList, Array.foldr_toList]
-      grind [GetElem?.getElem?, instGetElem?FixedExpZModMem]
-    · simp
-      unfold get?
-      rw [Array.foldr_toList, Array.foldr_toList]
-      grind
-
-end CircuitResult
+-- end CircuitResult
 
 namespace CircuitState
 
 variable {p : ℕ}
 
-def seq (circuit₁ circuit₂ : CircuitState p)
-        (varStore : VarStore p)
-        (numAlloc : ℕ) : CircuitResult p :=
-  let ⟨numAllocMid, varStoreMid, constraintsMid⟩ := eval circuit₁ varStore numAlloc
-  let ⟨numAllocPost, varStorePost, constraintsPost⟩ := eval circuit₂ varStoreMid numAllocMid
-  ⟨numAllocPost, varStorePost, constraintsMid ∧ constraintsPost⟩
+-- def seq (circuit₁ circuit₂ : CircuitState p)
+--         (varStore : VarStore p)
+--         (numAlloc : ℕ) : CircuitResult p :=
+--   let ⟨numAllocMid, varStoreMid, constraintsMid⟩ := eval circuit₁ varStore numAlloc
+--   let ⟨numAllocPost, varStorePost, constraintsPost⟩ := eval circuit₂ varStoreMid numAllocMid
+--   ⟨numAllocPost, varStorePost, constraintsMid ∧ constraintsPost⟩
 
-@[simp, grind=]
-lemma numAlloc_seq (circuit1 circuit2 : CircuitState p) (varStore : VarStore p) (numAlloc : ℕ):
-  (CircuitState.seq circuit1 circuit2 varStore numAlloc).numAlloc =
-  let mid := [varStore, numAlloc|circuit1]ₑ
-  [mid.varStore, mid.numAlloc|circuit2]ₑ.numAlloc
-:= rfl
+-- @[simp, grind=]
+-- lemma numAlloc_seq (circuit1 circuit2 : CircuitState p) (varStore : VarStore p) (numAlloc : ℕ):
+--   (CircuitState.seq circuit1 circuit2 varStore numAlloc).numAlloc =
+--   let mid := [varStore, numAlloc|circuit1]ₑ
+--   [mid.varStore, mid.numAlloc|circuit2]ₑ.numAlloc
+-- := rfl
 
-@[simp, grind=]
-lemma varStore_seq (circuit1 circuit2 : CircuitState p) (varStore : VarStore p) (numAlloc : ℕ):
-  (CircuitState.seq circuit1 circuit2 varStore numAlloc).varStore =
-  let mid := [varStore, numAlloc|circuit1]ₑ
-  [mid.varStore, mid.numAlloc|circuit2]ₑ.varStore
-:= rfl
+-- @[simp, grind=]
+-- lemma varStore_seq (circuit1 circuit2 : CircuitState p) (varStore : VarStore p) (numAlloc : ℕ):
+--   (CircuitState.seq circuit1 circuit2 varStore numAlloc).varStore =
+--   let mid := [varStore, numAlloc|circuit1]ₑ
+--   [mid.varStore, mid.numAlloc|circuit2]ₑ.varStore
+-- := rfl
 
-@[simp, grind=]
-lemma constraints_seq (circuit1 circuit2 : CircuitState p) (varStore : VarStore p) (numAlloc : ℕ):
-  (CircuitState.seq circuit1 circuit2 varStore numAlloc).constraints =
-  let mid := [varStore, numAlloc|circuit1]ₑ
-  mid.constraints ∧ [mid.varStore, mid.numAlloc|circuit2]ₑ.constraints
-:= rfl
+-- @[simp, grind=]
+-- lemma constraints_seq (circuit1 circuit2 : CircuitState p) (varStore : VarStore p) (numAlloc : ℕ):
+--   (CircuitState.seq circuit1 circuit2 varStore numAlloc).constraints =
+--   let mid := [varStore, numAlloc|circuit1]ₑ
+--   mid.constraints ∧ [mid.varStore, mid.numAlloc|circuit2]ₑ.constraints
+-- := rfl
 
-@[simp, grind =]
-lemma eval_append
-  {numAlloc}
-  {circuit1 circuit2 : CircuitState p}
-  {varStore}
-:
-  [varStore, numAlloc | circuit1 ++ circuit2]ₑ = seq circuit1 circuit2 varStore numAlloc
-:= by
-  simp [eval]
-  ext1
-  all_goals dsimp [seq]
-  . exact CircuitResult.foldl_step_numAlloc_independent_of_constraints
-  . exact CircuitResult.foldl_step_varStore_independent_of_constraints
-  . exact CircuitResult.foldl_step_constraints_and
+-- @[simp, grind =]
+-- lemma eval_append
+--   {numAlloc}
+--   {circuit1 circuit2 : CircuitState p}
+--   {varStore}
+-- :
+--   [varStore, numAlloc | circuit1 ++ circuit2]ₑ = seq circuit1 circuit2 varStore numAlloc
+-- := by
+--   simp [eval]
+--   ext1
+--   all_goals dsimp [seq]
+--   . exact CircuitResult.foldl_step_numAlloc_independent_of_constraints
+--   . exact CircuitResult.foldl_step_varStore_independent_of_constraints
+--   . exact CircuitResult.foldl_step_constraints_and
 
-@[simp high, grind =]
-lemma eval_singleton
-  {numAlloc}
-  {command : CircuitusPlanus p}
-  {varStore}
-:
-  [varStore, numAlloc | #[command]]ₑ =
-  [unconstrained[numAlloc][varStore] | command]ₛ := by
-  simp [eval, CircuitResult.step_unconstrained]
+-- @[simp high, grind =]
+-- lemma eval_singleton
+--   {numAlloc}
+--   {command : CircuitusPlanus p}
+--   {varStore}
+-- :
+--   [varStore, numAlloc | #[command]]ₑ =
+--   [unconstrained[numAlloc][varStore] | command]ₛ := by
+--   simp [eval, CircuitResult.step_unconstrained]
 
-@[simp, grind =]
-lemma eval_cons
-  {numAlloc}
-  {command : CircuitusPlanus p}
-  {circuit : CircuitState p}
-  {varStore}
-:
-  [varStore, numAlloc | ⟨command :: circuit.toList⟩]ₑ =
-  seq #[command] circuit varStore numAlloc := by
-  rw [show ⟨command :: circuit.toList⟩ = #[command] ++ circuit by simp]
-  exact eval_append
+-- @[simp, grind =]
+-- lemma eval_cons
+--   {numAlloc}
+--   {command : CircuitusPlanus p}
+--   {circuit : CircuitState p}
+--   {varStore}
+-- :
+--   [varStore, numAlloc | ⟨command :: circuit.toList⟩]ₑ =
+--   seq #[command] circuit varStore numAlloc := by
+--   rw [show ⟨command :: circuit.toList⟩ = #[command] ++ circuit by simp]
+--   exact eval_append
 
-section
+-- section
 
-variable {numAlloc : ℕ} {varStore : VarStore p} {e: FixedExp p}
+-- variable {numAlloc : ℕ} {varStore : VarStore p} {e: FixedExp p}
 
-@[simp, grind =]
-lemma eval_empty :
-  [varStore, numAlloc | #[]]ₑ = unconstrained[numAlloc][varStore]
-:= by rfl
+-- @[simp, grind =]
+-- lemma eval_empty :
+--   [varStore, numAlloc | #[]]ₑ = unconstrained[numAlloc][varStore]
+-- := by rfl
 
-@[simp, grind =]
-lemma eval_empty_collection :
-  [varStore, numAlloc | ∅]ₑ =
-  unconstrained[numAlloc][varStore]
-:= by rfl
+-- @[simp, grind =]
+-- lemma eval_empty_collection :
+--   [varStore, numAlloc | ∅]ₑ =
+--   unconstrained[numAlloc][varStore]
+-- := by rfl
 
-@[simp, grind =]
-lemma eval_eq0 :
-  [varStore, numAlloc | #[.eq0 e]]ₑ =
-  unconstrained[numAlloc][varStore].step (.eq0 e)
-:= by simp [eval, CircuitResult.addConstraint_unconstrained, GetElem?.getElem?]
+-- @[simp, grind =]
+-- lemma eval_eq0 :
+--   [varStore, numAlloc | #[.eq0 e]]ₑ =
+--   unconstrained[numAlloc][varStore].step (.eq0 e)
+-- := by simp [eval, CircuitResult.addConstraint_unconstrained, GetElem?.getElem?]
 
-@[simp, grind =]
-lemma eval_lam :
-  [varStore, numAlloc | #[.lam]]ₑ =
-  unconstrained[numAlloc][varStore].step (.lam)
-:= by
-  simp [eval]
+-- @[simp, grind =]
+-- lemma eval_lam :
+--   [varStore, numAlloc | #[.lam]]ₑ =
+--   unconstrained[numAlloc][varStore].step (.lam)
+-- := by
+--   simp [eval]
 
-@[simp, grind =]
-lemma eval_share :
-  [varStore, numAlloc | #[.share e]]ₑ =
-  unconstrained[numAlloc][varStore].step (.share e)
-:= by
-  simp [eval, CircuitResult.addConstraint_unconstrained, Membership.mem]
+-- @[simp, grind =]
+-- lemma eval_share :
+--   [varStore, numAlloc | #[.share e]]ₑ =
+--   unconstrained[numAlloc][varStore].step (.share e)
+-- := by
+--   simp [eval, CircuitResult.addConstraint_unconstrained, Membership.mem]
 
-@[simp, grind =]
-lemma eval_isZero :
-  [varStore, numAlloc | #[.isZero e]]ₑ =
-  unconstrained[numAlloc][varStore].step (.isZero e)
-:= by
-  simp [eval, CircuitResult.addConstraint_unconstrained, Membership.mem]
-  rfl
+-- @[simp, grind =]
+-- lemma eval_isZero :
+--   [varStore, numAlloc | #[.isZero e]]ₑ =
+--   unconstrained[numAlloc][varStore].step (.isZero e)
+-- := by
+--   simp [eval, CircuitResult.addConstraint_unconstrained, Membership.mem]
+--   rfl
 
-@[simp, grind =]
-lemma eval_num2bits {width : ℕ} :
-  [varStore, numAlloc | #[.num2bits width e]]ₑ =
-  unconstrained[numAlloc][varStore].step (.num2bits width e)
-:= by
-  simp [eval, CircuitResult.addConstraint_unconstrained, Membership.mem, GetElem?.getElem!]
+-- @[simp, grind =]
+-- lemma eval_num2bits {width : ℕ} :
+--   [varStore, numAlloc | #[.num2bits width e]]ₑ =
+--   unconstrained[numAlloc][varStore].step (.num2bits width e)
+-- := by
+--   simp [eval, CircuitResult.addConstraint_unconstrained, Membership.mem, GetElem?.getElem!]
 
-@[simp, grind =]
-lemma seq_cons_nil {cmd : CircuitusPlanus p} {circuit : CircuitState p} {varStore} {numAlloc} :
-  seq (⟨cmd :: circuit.toList⟩) #[] varStore numAlloc =
-  seq #[cmd] circuit varStore numAlloc := by
-  aesop (add simp seq)
+-- @[simp, grind =]
+-- lemma seq_cons_nil {cmd : CircuitusPlanus p} {circuit : CircuitState p} {varStore} {numAlloc} :
+--   seq (⟨cmd :: circuit.toList⟩) #[] varStore numAlloc =
+--   seq #[cmd] circuit varStore numAlloc := by
+--   aesop (add simp seq)
 
-@[simp high, grind =]
-lemma seq_singleton_nil {cmd : CircuitusPlanus p} {varStore} {numAlloc} :
-  seq #[cmd] #[] varStore numAlloc =
-  [varStore, numAlloc| #[cmd]]ₑ := by
-  simp [seq]
+-- @[simp high, grind =]
+-- lemma seq_singleton_nil {cmd : CircuitusPlanus p} {varStore} {numAlloc} :
+--   seq #[cmd] #[] varStore numAlloc =
+--   [varStore, numAlloc| #[cmd]]ₑ := by
+--   simp [seq]
 
-end
+-- end
 
 end CircuitState
 
-end Edsl
+-- end Edsl
 
-end Clap
+-- end Clap
