Clap/eDSLState/HashCons/Eval.lean
@@ -26,7 +26,7 @@ def evalAux {p}
       -- for leaves, insert their value, looking at the varstore if needed
       | .c value => cache.insert e (.some value)
       | .v idx => cache.insert e (Γ.get? idx)
-      -- for branch nodes, recurse, adding the children's values if needed
+      -- for branch nodes, recurse, adding the childrens' values if needed
       | .binary_op lhs rhs op =>
         have lhs_precedes_your_index : lhs < e := by
           grind [HashConsSt.wellFormed, CacheExpr.wellFormed]
@@ -163,27 +163,43 @@ lemma runGet_mkMul {l r : ExprRef} (h: (CacheExpr.binary_op (p := p) l r BinaryO
 attribute [local grind ext]
   Option.ext Prod.ext Id.ext
 
+abbrev val {α} (a : HashConsM p α) (σ : HashConsSt p) := (a.run σ).1
+
+abbrev st {α} (a : HashConsM p α) (σ : HashConsSt p) := (a.run σ).2
+
 lemma eval_run_of_runGet?_eq_some_c {ref : HashConsM p ExprRef}
-           (h : ref.runGet? σ = .some (.c k)) :
-  [varStore,σ|ref] = (.some k, (ref.run σ).2) := by
+        (h : ref.runGet? σ = .some (.c k)) :
+  [varStore,σ|ref] = (.some k, ref.st σ) := by
   simp [eval]
   grind [=Id.run, Functor.map]
 
+def ValueCache.wellFormed {p} (Γ : VarStore p) (σ : HashConsSt p) (cache : ValueCache p) : Prop :=
+  ∀ (e : ExprRef) (r : Option (ZMod p)),
+    cache[e]? = .some r → (evalAux Γ e ∅ σ)[e]? = r
+
+theorem ValueCahcke.wellFormed_evalAux_of_wellFormed {Γ : VarStore p} {e}
+  (h : ValueCache.wellFormed Γ σ cache) : ValueCache.wellFormed Γ σ (evalAux Γ e cache σ) := by
+  sorry    
+
 -- TODO move evalAux into hypothesis?
 -- TODO generalise to wellFormed cache
-lemma eval_run_pure {k : ExprRef}:
-  [varStore,σ|pure k] = ((evalAux varStore k {} σ)[k]?.join, σ)
-:= rfl
+lemma eval_run_pure {k : ExprRef} {cache : ValueCache p} (h : cache.wellFormed varStore σ) :
+  [varStore,σ|pure k] = ((evalAux varStore k cache σ)[k]?.join, σ)
+:= by
+  unfold eval
+  suffices (evalAux varStore k ∅ σ)[k]?.join = (evalAux varStore k cache σ)[k]?.join by simpa
+  
+  
 
 lemma eval_run_bind {α} {a : HashConsM p α} {f : α → HashConsM p ExprRef} :
-  [varStore,σ|a >>= f] =
-  [varStore,(a.run σ).2|f (a.run σ).1]
+  [varStore, σ|a >>= f] =
+  [varStore, a.st σ|f (a.val σ)]
 := rfl
 
 -- TODO, this is really just idxOf∧contains=>get?=.some, and get?=runGet?
 lemma run_eval_idxOf_c_of_contains {ref : HashConsM p ExprRef} {e : CacheExpr p}
-  (h : (ref.run σ).2.exprs.contains e)
-  (h': (ref.run σ).1 = (ref.run σ).2.exprs.idxOf e)
+  (h₁ : e ∈ (ref.st σ).exprs)
+  (h₂ : ref.val σ = (ref.st σ).exprs.idxOf e)
 :
   ref.runGet? σ = .some e
 := by
@@ -191,8 +207,8 @@ lemma run_eval_idxOf_c_of_contains {ref : HashConsM p ExprRef} {e : CacheExpr p}
 
 @[grind .]
 lemma run_eval_idxOf_c_of_contains' {ref : HashConsM p ExprRef} {e : CacheExpr p}
-  (h : (ref σ).2.exprs.contains e)
-  (h': (ref σ).1 = (ref σ).2.exprs.idxOf e)
+  (h : e ∈ (ref.st σ).exprs)
+  (h': ref.val σ = (ref.st σ).exprs.idxOf e)
 :
   ref.runGet? σ = .some e
 := run_eval_idxOf_c_of_contains h h'
@@ -203,42 +219,41 @@ lemma HashConsSt.exprs_mem_pushExpr {e : CacheExpr p} (h : e.wellFormed σ.exprs
   simp [HashConsSt.pushExpr]
 
 lemma eval_pushExpr {ref : HashConsM p ExprRef}
-  (h : ref.run' (σ.pushExpr (.c k) wellFormed_c) = σ.exprs.size)
+  (h : ref.val (σ.pushExpr (.c k) wellFormed_c) = σ.exprs.size)
 :
-  ([varStore|ref].run (σ.pushExpr (.c k) wellFormed_c)).run =
-  (.some k, (ref.run σ).run.2)
+  [varStore, σ.pushExpr (.c k) wellFormed_c|ref] = (.some k, ref.st σ)
 := by
-  simp
+  sorry
+  
+-- @[simp, grind =]
+-- lemma run_mkConstant_eval_c_of_mem
+--   {p : ℕ}
+--   {k : ZMod p}
+--   {varStore : VarStore p}
+--   {σ : HashConsSt p}
+--   (h : .c k ∈ σ.exprs)
+-- :
+--   (mkConstant k >>= ([varStore|·])).run σ = (.some k, σ)
+-- := by
+--   simp
+--   simp [StateT.run, h]
+--   unfold_projs
+--   grind
 
-@[simp, grind =]
-lemma run_mkConstant_eval_c_of_mem
-  {p : ℕ}
-  {k : ZMod p}
-  {varStore : VarStore p}
-  {σ : HashConsSt p}
-  (h : .c k ∈ σ.exprs)
-:
-  (mkConstant k >>= ([varStore|·])).run σ = (.some k, σ)
-:= by
-  simp
-  simp [StateT.run, h]
-  unfold_projs
-  grind
-
-@[simp, grind =]
-lemma run_mkConstant_eval_c_of_notMem
-  {p : ℕ}
-  {k : ZMod p}
-  {varStore : VarStore p}
-  {σ : HashConsSt p}
-  (h : .c k ∉ σ.exprs)
-:
-  (mkConstant k >>= ([varStore|·])).run σ = (.some k, σ.pushExpr (.c k) sorry)
-:= by
-  simp
-  simp [StateT.run, h]
-  unfold_projs
-  simp
+-- @[simp, grind =]
+-- lemma run_mkConstant_eval_c_of_notMem
+--   {p : ℕ}
+--   {k : ZMod p}
+--   {varStore : VarStore p}
+--   {σ : HashConsSt p}
+--   (h : .c k ∉ σ.exprs)
+-- :
+--   (mkConstant k >>= ([varStore|·])).run σ = (.some k, σ.pushExpr (.c k) sorry)
+-- := by
+--   simp
+--   simp [StateT.run, h]
+--   unfold_projs
+--   simp
 
 
 end
@@ -250,157 +265,165 @@ lemma eval_c
   {varStore : VarStore p}
   {σ : HashConsSt p}
 :
-  [varStore,σ|mkConstant k] = some k
+  [varStore,σ|mkConstant k] =
+  (
+    .some k,
+    if CacheExpr.c k ∈ σ.exprs
+    then σ
+    else HashConsSt.pushExpr (CacheExpr.c k) σ wellFormed_c
+  )
 := by
-  simp [eval]
-  aesop (add simp [Functor.map]) (add safe (by grind))
+  unfold eval
+  simp
+  
+  -- aesop (add simp [Functor.map]) (add safe (by grind))
 
-@[simp, grind .]
-lemma eval_ofNat {p n : ℕ} {varStore : VarStore p} :
-  [varStore|no_index (OfNat.ofNat n)] = .some n := by
-  simp [FixedExp.eval]
-
-@[simp, grind =]
-lemma eval_v
-  {p : ℕ}
-  {varIdx : ℕ}
-  {varStore : VarStore p}
-:
-  [varStore|Exp.v varIdx] = varStore[varIdx]?
-:= by
-  simp [FixedExp.eval]
-
-@[simp, grind =]
-lemma add_def
-  {p : ℕ}
-  {a b : FixedExp p}
-:
-  a + b =
-  Exp.add a b
-:= by
-  simp [HAdd.hAdd, Add.add]
+-- @[simp, grind .]
+-- lemma eval_ofNat {p n : ℕ} {varStore : VarStore p} :
+--   [varStore|no_index (OfNat.ofNat n)] = .some n := by
+--   simp [FixedExp.eval]
 
 -- @[simp, grind =]
-@[grind =]
-lemma sub_def
-  {p : ℕ}
-  {a b : FixedExp p}
-:
-  a - b =
-  Exp.sub a b
-:= by
-  simp [HSub.hSub, Sub.sub]
+-- lemma eval_v
+--   {p : ℕ}
+--   {varIdx : ℕ}
+--   {varStore : VarStore p}
+-- :
+--   [varStore|Exp.v varIdx] = varStore[varIdx]?
+-- := by
+--   simp [FixedExp.eval]
 
-@[simp, grind =]
-lemma mul_def
-  {p : ℕ}
-  {a b : FixedExp p}
-:
-  a * b =
-  Exp.mul a b
-:= by
-  simp [HMul.hMul, Mul.mul]
+-- @[simp, grind =]
+-- lemma add_def
+--   {p : ℕ}
+--   {a b : FixedExp p}
+-- :
+--   a + b =
+--   Exp.add a b
+-- := by
+--   simp [HAdd.hAdd, Add.add]
 
-@[simp, grind =]
-lemma eval_add
-  {p : ℕ}
-  {varStore : VarStore p}
-  {a b : FixedExp p}
-:
-  [varStore|Exp.add a b] =
-  (do (←eval varStore a) + (←eval varStore b))
-:= rfl
+-- -- @[simp, grind =]
+-- @[grind =]
+-- lemma sub_def
+--   {p : ℕ}
+--   {a b : FixedExp p}
+-- :
+--   a - b =
+--   Exp.sub a b
+-- := by
+--   simp [HSub.hSub, Sub.sub]
 
-@[grind .]
-lemma eval_none_add
-  {p : ℕ}
-  {varStore : VarStore p}
-  {a b : FixedExp p}
-  (h : [varStore|a] = .none)
-:
-  [varStore|Exp.add a b] =
-  .none
-:= by
-  simp [FixedExp.eval, h]
+-- @[simp, grind =]
+-- lemma mul_def
+--   {p : ℕ}
+--   {a b : FixedExp p}
+-- :
+--   a * b =
+--   Exp.mul a b
+-- := by
+--   simp [HMul.hMul, Mul.mul]
 
-@[grind .]
-lemma eval_add_none
-  {p : ℕ}
-  {varStore : VarStore p}
-  {a b : FixedExp p}
-  (h : [varStore|b] = .none)
-:
-  [varStore|Exp.add a b] =
-  .none
-:= by
-  simp [FixedExp.eval, h]
+-- @[simp, grind =]
+-- lemma eval_add
+--   {p : ℕ}
+--   {varStore : VarStore p}
+--   {a b : FixedExp p}
+-- :
+--   [varStore|Exp.add a b] =
+--   (do (←eval varStore a) + (←eval varStore b))
+-- := rfl
 
-@[simp, grind =]
-lemma eval_sub
-  {p : ℕ}
-  {varStore : VarStore p}
-  {a b : FixedExp p}
-:
-  [varStore|Exp.sub a b] =
-  (do (←eval varStore a) - (←eval varStore b))
-:= rfl
+-- @[grind .]
+-- lemma eval_none_add
+--   {p : ℕ}
+--   {varStore : VarStore p}
+--   {a b : FixedExp p}
+--   (h : [varStore|a] = .none)
+-- :
+--   [varStore|Exp.add a b] =
+--   .none
+-- := by
+--   simp [FixedExp.eval, h]
 
-@[grind .]
-lemma eval_none_sub
-  {p : ℕ}
-  {varStore : VarStore p}
-  {a b : FixedExp p}
-  (h : [varStore|a] = .none)
-:
-  [varStore|Exp.sub a b] =
-  .none
-:= by
-  simp [FixedExp.eval, h]
+-- @[grind .]
+-- lemma eval_add_none
+--   {p : ℕ}
+--   {varStore : VarStore p}
+--   {a b : FixedExp p}
+--   (h : [varStore|b] = .none)
+-- :
+--   [varStore|Exp.add a b] =
+--   .none
+-- := by
+--   simp [FixedExp.eval, h]
 
-@[grind .]
-lemma eval_sub_none
-  {p : ℕ}
-  {varStore : VarStore p}
-  {a b : FixedExp p}
-  (h : [varStore|b] = .none)
-:
-  [varStore|Exp.sub a b] =
-  .none
-:= by
-  simp [FixedExp.eval, h]
+-- @[simp, grind =]
+-- lemma eval_sub
+--   {p : ℕ}
+--   {varStore : VarStore p}
+--   {a b : FixedExp p}
+-- :
+--   [varStore|Exp.sub a b] =
+--   (do (←eval varStore a) - (←eval varStore b))
+-- := rfl
 
-@[simp, grind =]
-lemma eval_mul
-  {p : ℕ}
-  {varStore : VarStore p}
-  {a b : FixedExp p}
-:
-  [varStore|Exp.mul a b] =
-  (do (←eval varStore a) * (←eval varStore b))
-:= rfl
+-- @[grind .]
+-- lemma eval_none_sub
+--   {p : ℕ}
+--   {varStore : VarStore p}
+--   {a b : FixedExp p}
+--   (h : [varStore|a] = .none)
+-- :
+--   [varStore|Exp.sub a b] =
+--   .none
+-- := by
+--   simp [FixedExp.eval, h]
 
-@[grind .]
-lemma eval_none_mul
-  {p : ℕ}
-  {varStore : VarStore p}
-  {a b : FixedExp p}
-  (h : [varStore|a] = .none)
-:
-  [varStore|Exp.mul a b] =
-  .none
-:= by
-  simp [FixedExp.eval, h]
+-- @[grind .]
+-- lemma eval_sub_none
+--   {p : ℕ}
+--   {varStore : VarStore p}
+--   {a b : FixedExp p}
+--   (h : [varStore|b] = .none)
+-- :
+--   [varStore|Exp.sub a b] =
+--   .none
+-- := by
+--   simp [FixedExp.eval, h]
 
-@[grind .]
-lemma eval_mul_none
-  {p : ℕ}
-  {varStore : VarStore p}
-  {a b : FixedExp p}
-  (h : [varStore|b] = .none)
-:
-  [varStore|Exp.mul a b] =
-  .none
-:= by
-  simp [FixedExp.eval, h]
+-- @[simp, grind =]
+-- lemma eval_mul
+--   {p : ℕ}
+--   {varStore : VarStore p}
+--   {a b : FixedExp p}
+-- :
+--   [varStore|Exp.mul a b] =
+--   (do (←eval varStore a) * (←eval varStore b))
+-- := rfl
+
+-- @[grind .]
+-- lemma eval_none_mul
+--   {p : ℕ}
+--   {varStore : VarStore p}
+--   {a b : FixedExp p}
+--   (h : [varStore|a] = .none)
+-- :
+--   [varStore|Exp.mul a b] =
+--   .none
+-- := by
+--   simp [FixedExp.eval, h]
+
+-- @[grind .]
+-- lemma eval_mul_none
+--   {p : ℕ}
+--   {varStore : VarStore p}
+--   {a b : FixedExp p}
+--   (h : [varStore|b] = .none)
+-- :
+--   [varStore|Exp.mul a b] =
+--   .none
+-- := by
+--   simp [FixedExp.eval, h]
 
 end Clap.HashConsM
