Clap/eDSLState/Monad.lean
@@ -37,65 +37,69 @@ lemma CircuitState.one_eq_nil :
 
 end Monoid
 
-namespace CircuitStateM
-
-def run {p : ℕ} {α : Type} (cmd : CircuitStateM p α) (numAlloc : ℕ) :=
+def CircuitStateM.run {p : ℕ} {α : Type} (cmd : ClapM p α) (numAlloc : ℕ) :=
   StateT.run (WriterT.run cmd) numAlloc
 
+namespace ClapM
+
+def run {p : ℕ} {α : Type} (cmd : ClapM p α) (numAlloc : ℕ) (σ : HashConsSt p) :
+  ((α × CircuitState p) × ℕ) × HashConsSt p :=
+  (StateT.run (WriterT.run cmd) numAlloc).run σ
+
 @[simp, grind =]
-lemma run_def {α} {cmd : CircuitStateM p α} {numAlloc} :
-  CircuitStateM.run cmd numAlloc = cmd numAlloc := rfl
+lemma run_def {α} {cmd : ClapM p α} {numAlloc} :
+  ClapM.run cmd numAlloc = cmd numAlloc := rfl
 
 def runAndEval
-  {p : ℕ} {α : Type} (cmd : CircuitStateM p α) (numAlloc : ℕ) (varStore : VarStore p)
+  {p : ℕ} {α : Type} (cmd : ClapM p α) (numAlloc : ℕ) (varStore : VarStore p) (σ : HashConsSt p)
 :
   α × CircuitResult p
 :=
-  let ⟨⟨result, circuit⟩, _numAlloc⟩ := cmd.run numAlloc
+  let ⟨⟨⟨result, circuit⟩, _numAlloc⟩, _σ⟩ := cmd.run numAlloc σ
   ⟨result, Edsl.CircuitState.eval circuit varStore numAlloc⟩
 
-def alloc {p : ℕ} : CircuitStateM p ℕ :=
+def alloc {p : ℕ} : ClapM p ℕ :=
   getModify (· + 1)
 
 section Getters
 
 abbrev getResult
-  {p : ℕ} {α : Type} (cmd : CircuitStateM p α) (numAlloc : ℕ)
+  {p : ℕ} {α : Type} (cmd : ClapM p α) (numAlloc : ℕ)
 : α :=
   (cmd.run numAlloc).1.1
 
 abbrev getCircuit
-  {p : ℕ} {α : Type} (cmd : CircuitStateM p α) (numAlloc : ℕ)
+  {p : ℕ} {α : Type} (cmd : ClapM p α) (numAlloc : ℕ)
 : CircuitState p :=
   (cmd.run numAlloc).1.2
 
 abbrev getNumAlloc
-  {p : ℕ} {α : Type} (cmd : CircuitStateM p α) (numAlloc : ℕ)
+  {p : ℕ} {α : Type} (cmd : ClapM p α) (numAlloc : ℕ)
 : ℕ :=
   (cmd.run numAlloc).2
 
 @[simp, grind=]
 lemma getResult_alloc (numAlloc : ℕ):
-  (CircuitStateM.alloc (p := p)).getResult numAlloc =
+  (ClapM.alloc (p := p)).getResult numAlloc =
   numAlloc
 := rfl
 
 @[simp, grind=]
 lemma getCircuit_alloc (numAlloc : ℕ):
-  (CircuitStateM.alloc (p := p)).getCircuit numAlloc =
+  (ClapM.alloc (p := p)).getCircuit numAlloc =
   #[]
 := rfl
 
 @[simp, grind=]
 lemma getNumAlloc_alloc (numAlloc : ℕ):
-  (CircuitStateM.alloc (p := p)).getNumAlloc numAlloc = numAlloc + 1
+  (ClapM.alloc (p := p)).getNumAlloc numAlloc = numAlloc + 1
 := rfl
 
 @[simp, grind =]
 lemma getResult_bind
   {α β}
-  {action : CircuitStateM p α}
-  {function : α → CircuitStateM p β}
+  {action : ClapM p α}
+  {function : α → ClapM p β}
   {numAlloc : ℕ}
 :
   (action >>= function).getResult numAlloc =
@@ -105,8 +109,8 @@ lemma getResult_bind
 @[simp, grind =]
 lemma getCircuit_bind
   {α β}
-  {action : CircuitStateM p α}
-  {function : α → CircuitStateM p β}
+  {action : ClapM p α}
+  {function : α → ClapM p β}
   {numAlloc : ℕ}
 :
   (action >>= function).getCircuit numAlloc =
@@ -117,8 +121,8 @@ lemma getCircuit_bind
 @[simp, grind =]
 lemma getNumAlloc_bind
   {α β}
-  {action : CircuitStateM p α}
-  {function : α → CircuitStateM p β}
+  {action : ClapM p α}
+  {function : α → ClapM p β}
   {numAlloc : ℕ}
 :
   (action >>= function).getNumAlloc numAlloc =
@@ -127,53 +131,53 @@ lemma getNumAlloc_bind
 
 @[simp, grind =]
 lemma getResult_tell (numAlloc : ℕ) (xs : CircuitState p):
-  CircuitStateM.getResult (tell xs) numAlloc = ()
+  ClapM.getResult (tell xs) numAlloc = ()
 := rfl
 
 @[simp, grind =]
 lemma getCircuit_tell (numAlloc : ℕ) (xs : CircuitState p):
-  CircuitStateM.getCircuit (tell xs) numAlloc =
+  ClapM.getCircuit (tell xs) numAlloc =
   xs
 := rfl
 
 @[simp, grind =]
 lemma getNumAlloc_tell (numAlloc : ℕ) (xs : CircuitState p):
-  CircuitStateM.getNumAlloc (tell xs) numAlloc =
+  ClapM.getNumAlloc (tell xs) numAlloc =
   numAlloc
 := rfl
 
 @[simp, grind=]
 lemma getResult_pure {α} (numAlloc : ℕ) (x : α):
-  CircuitStateM.getResult (p := p) (pure x) numAlloc =
+  ClapM.getResult (p := p) (pure x) numAlloc =
   x
 := rfl
 
 @[simp, grind=]
 lemma getCircuit_pure {α} (numAlloc : ℕ) (x : α):
-  CircuitStateM.getCircuit (p := p) (pure x) numAlloc =
+  ClapM.getCircuit (p := p) (pure x) numAlloc =
   #[]
 := rfl
 
 @[simp, grind=]
 lemma getNumAlloc_pure {α} (numAlloc : ℕ) (x : α) :
-  CircuitStateM.getNumAlloc (p := p) (pure x) numAlloc =
+  ClapM.getNumAlloc (p := p) (pure x) numAlloc =
   numAlloc
 := rfl
 
 @[simp, grind=]
-lemma getResult_map {α β} (f : α → β) (numAlloc : ℕ) (cmd : CircuitStateM p α):
+lemma getResult_map {α β} (f : α → β) (numAlloc : ℕ) (cmd : ClapM p α):
   (f <$> cmd).getResult numAlloc =
   f (cmd.getResult numAlloc)
 := rfl
 
 @[simp, grind=]
-lemma getNumAlloc_map {α β} (f : α → β) (numAlloc : ℕ) (cmd : CircuitStateM p α):
+lemma getNumAlloc_map {α β} (f : α → β) (numAlloc : ℕ) (cmd : ClapM p α):
   (f <$> cmd).getNumAlloc numAlloc =
   (cmd.getNumAlloc) numAlloc
 := rfl
 
 @[simp, grind=]
-lemma getCircuit_map {α β} (f : α → β) (numAlloc : ℕ) (cmd : CircuitStateM p α):
+lemma getCircuit_map {α β} (f : α → β) (numAlloc : ℕ) (cmd : ClapM p α):
   (f <$> cmd).getCircuit numAlloc =
   (cmd.getCircuit) numAlloc
 := rfl
@@ -182,7 +186,7 @@ end Getters
 
 def wellFormed
   {α : Type}
-  (action : CircuitStateM p α)
+  (action : ClapM p α)
 :
   Prop
 :=
@@ -190,13 +194,13 @@ def wellFormed
     (action.getNumAlloc numAlloc) =
     (CircuitState.eval (action.getCircuit numAlloc) varStore numAlloc).numAlloc
 
-end CircuitStateM
+end ClapM
 
 attribute [Clap.monads, grind =]
   bind
   pure
 
-  CircuitStateM.run
+  ClapM.run
 
   WriterT.run
   WriterT.mk
@@ -217,8 +221,8 @@ lemma eval_bind
   {α β : Type}
   {varStore : VarStore p}
   {numAlloc : ℕ}
-  {action : CircuitStateM p α}
-  {function : α → CircuitStateM p β}
+  {action : ClapM p α}
+  {function : α → ClapM p β}
 :
   eval ((action >>= function).getCircuit numAlloc) varStore numAlloc =
   let ((result, action_circuit), numAlloc') := action.run numAlloc
@@ -231,8 +235,8 @@ lemma runAndEval_bind
   {α β : Type}
   {varStore : VarStore p}
   {numAlloc : ℕ}
-  {action : CircuitStateM p α}
-  {function : α → CircuitStateM p β}
+  {action : ClapM p α}
+  {function : α → ClapM p β}
   (h_wf : action.wellFormed)
 :
   (action >>= function).runAndEval numAlloc varStore =
@@ -241,9 +245,9 @@ lemma runAndEval_bind
   ⟨functionData, functionCircuitResult.addConstraint actionCircuitResult.constraints⟩
 := by
   sorry
-  -- simp [CircuitStateM.runAndEval, Clap.monads]
+  -- simp [ClapM.runAndEval, Clap.monads]
   -- have : (eval (action numAlloc).1.2 varStore numAlloc).numAlloc = (action numAlloc).2 := by
-  --   simp [CircuitStateM.wellFormed, Clap.monads] at h_wf
+  --   simp [ClapM.wellFormed, Clap.monads] at h_wf
   --   exact (h_wf numAlloc varStore).symm
   -- set x := action numAlloc
   -- obtain ⟨a, b⟩ := x
@@ -254,7 +258,7 @@ lemma runAndEval_bind
 
 end CircuitState
 
-namespace CircuitStateM
+namespace ClapM
 
 section
 
@@ -266,18 +270,18 @@ lemma getModify_eq
 :
   @getModify
     ℕ
-    (CircuitStateM p)
-    (instMonadStateOfMonadStateOf ℕ (CircuitStateM p))
+    (ClapM p)
+    (instMonadStateOfMonadStateOf ℕ (ClapM p))
     f
     numAlloc = ((numAlloc, #[]), f numAlloc)
 := rfl
 
 @[simp, grind =]
 lemma alloc_eq :
-  CircuitStateM.alloc (p := p) numAlloc =
+  ClapM.alloc (p := p) numAlloc =
   ((numAlloc, #[]), numAlloc + 1)
 := by
-  simp [CircuitStateM.alloc, Clap.monads]
+  simp [ClapM.alloc, Clap.monads]
 
 @[Clap.monads]
 lemma Vector_ofFnM_empty_state
@@ -286,7 +290,7 @@ lemma Vector_ofFnM_empty_state
   {a : Fin n → ℕ → α}
   {c : Fin n → ℕ → ℕ}
 :
-  (@Vector.ofFnM (CircuitStateM p) _ n _ (λ x s => ⟨⟨a x s, #[]⟩, c x s⟩) numAlloc).1.2 =
+  (@Vector.ofFnM (ClapM p) _ n _ (λ x s => ⟨⟨a x s, #[]⟩, c x s⟩) numAlloc).1.2 =
   #[]
 := by
   induction n with
@@ -295,7 +299,7 @@ lemma Vector_ofFnM_empty_state
   | succ n h =>
     rewrite [Vector.ofFnM_succ]
     simp_all [Clap.monads]
-    set x := @Vector.ofFnM (CircuitStateM p) _ _ _ _ _
+    set x := @Vector.ofFnM (ClapM p) _ _ _ _ _
     have : x = ⟨x.1, x.2⟩ := rfl
     rewrite [this]; clear this
     simp [x, h]
@@ -313,7 +317,7 @@ lemma bind_eval' {α} {a} {varStore : VarStore p} {f : ZMod p → Option α} (h 
 
 end
 
-end CircuitStateM
+end ClapM
 
 end Edsl
 
